First version of automation running

icing/examples/exampleLib.sml
@@ -608,6 +608,421 @@ struct
                    |> #1 (* take the list, ignore type *)
   val stos_pass_correct_thm = save_thm ("stos_pass_correct_thm", mk_stos_pass_correct_thm plan_list)
   val stos_pass_real_id_thm = save_thm ("stos_pass_real_id_thm", mk_stos_pass_real_id_thm plan_list)
+  val main_spec_thm =
+    if (not checkError) then CONJ_COMM
+    else
+      let
+      val st = get_ml_prog_state ();
+      (* Precreate terms for arguments *)
+      val (args, argList, vList) =
+        if numArgs = 1 then (“(w1):word64”, “[w1]:word64 list”, “[d1]:v list”)
+        else if numArgs = 2 then (“(w1, w2):word64 # word64”, “[w1;w2]:word64 list”, “[d1; d2]:v list”)
+        else if numArgs = 3 then (“(w1, w2, w3):word64 # word64 # word64”,
+                                  “[w1; w2; w3]:word64 list”,
+                                  “[d1; d2; d3]:v list”)
+        else if numArgs = 4 then
+          (“(w1, w2, w3, w4):word64 # word64 # word64 #word64”,
+           “[w1; w2; w3; w4]:word64 list”,
+           “[d1; d2; d3; d4]:v list”)
+        else if numArgs = 6 then
+          (“(w1, w2, w3, w4, w5, w6):word64 # word64 # word64 # word64 # word64 #word64”,
+           “[w1; w2; w3; w4; w5; w6]:word64 list”,
+           “[d1; d2; d3; d4; d5; d6]:v list”)
+        else if numArgs = 8 then
+          (“(w1, w2, w3, w4, w5, w6, w7, w8):word64#word64#word64#word64#word64#word64#word64#word64”,
+           “[w1; w2; w3; w4; w5; w6; w7; w8]:word64 list”,
+           “[d1; d2; d3; d4; d5; d6; d7; d8]:v list”)
+        else (“(w1, w2, w3, w4, w5, w6, w7, w8, w9):
+                word64#word64#word64#word64#word64#word64#word64#word64#word64”,
+              “[w1; w2; w3; w4; w5; w6; w7; w8; w9]:word64 list”,
+              “[d1; d2; d3; d4; d5; d6; d7; d8; d9]:v list”)
+      (* Define a real-number and floating-point spec*)
+      val theAST_real_spec_def =
+        Define ‘theAST_real_spec ^args = real_spec_prog ^body_opt theAST_env ^fvars ^argList’
+      val theAST_opt_float_option_noopt_def =
+        Define ‘theAST_opt_float_option_noopt ^args =
+                case evaluate
+                     (empty_state with fp_state := empty_state.fp_state with canOpt := FPScope NoOpt)
+                     (theAST_env with v :=
+                        extend_env_with_vars (REVERSE ^fvars) (REVERSE ^argList) (theAST_env).v)
+                [^body_opt] of
+                | (st, Rval [FP_WordTree fp]) =>
+                  if st = (empty_state with fp_state := empty_state.fp_state
+                    with canOpt := FPScope NoOpt)
+                  then SOME fp else NONE
+                | _ => NONE’
+      val theAST_opt_float_option_def =
+        Define ‘theAST_opt_float_option ^args =
+               case evaluate empty_state
+                      (theAST_env with v :=
+                        extend_env_with_vars (REVERSE ^fvars) (REVERSE ^argList) (theAST_env).v)
+               [^body_opt] of
+               | (st, Rval [FP_WordTree fp]) => if (st = empty_state) then SOME fp else NONE
+               | _ => NONE’
+      val theAST_float_returns_def =
+        Define ‘
+        theAST_float_returns ^args w ⇔
+        ∃ fpOpts st2 fp.
+          let theOpts = FLAT (MAP (λ x. case x of |Apply (_, rws) => rws |_ => []) (HD theAST_plan)) in
+            evaluate (empty_state with fp_state :=
+                      empty_state.fp_state with
+                                 <| rws := theOpts ; opts := fpOpts; canOpt := FPScope NoOpt |>)
+                     (theAST_env with v :=
+                      extend_env_with_vars (REVERSE ^fvars) (REVERSE ^argList) (theAST_env).v)
+                     [^body] = (st2, Rval [FP_WordTree fp]) ∧ compress_word fp = w’
+      val freeVars_list_body = store_thm ("freeVars_list_body",
+        Parse.Term ‘
+        ∀ (st1:unit semanticPrimitives$state) st2.
+          freeVars_list_arithExp_bound
+            st1 st2 [^body]
+            (theAST_env with v :=
+             extend_env_with_vars (REVERSE ^fvars) (REVERSE ^argList) (theAST_env).v)’,
+        rpt strip_tac
+        \\ gs[freeVars_arithExp_bound_def, icing_rewriterTheory.isFpArithExp_def,
+              freeVars_fp_bound_def]
+        \\ rpt conj_tac
+        (* Non-let goals are automatically solved *)
+        \\ TRY (gs[extend_env_with_vars_def] \\ NO_TAC)
+        (* Remainder: let-goals *)
+        \\ rpt strip_tac
+        (* Let-goals not reasoning about let-bound variable *)
+        \\ TRY (gs[extend_env_with_vars_def,namespaceTheory.nsOptBind_def] \\ NO_TAC)
+        \\ rveq
+        \\ qpat_x_assum ‘evaluate _ _ _ = _’ mp_tac
+        \\ qmatch_goalsub_abbrev_tac ‘evaluate theState theEnv [theExp] = _’
+        \\ ‘isFpArithExp theExp’ by (unabbrev_all_tac \\ EVAL_TAC)
+        \\ first_x_assum $ mp_then Any mp_tac (INST_TYPE [“:'a” |-> “:unit”]
+                (CONJUNCT1 icing_rewriterProofsTheory.isFpArithExp_matched_evaluates))
+        \\ disch_then (qspecl_then [‘theEnv’, ‘theState’] mp_tac)
+        \\ impl_tac
+        (* free variables must be bound *)
+        \\ TRY (rpt strip_tac \\ rename1 ‘x IN FV theExp’ \\ unabbrev_all_tac
+                \\ gs[extend_env_with_vars_def, namespaceTheory.nsOptBind_def]
+                \\ NO_TAC)
+        (* use the theorem to prove the conclusion *)
+        \\ TRY (rpt strip_tac \\ imp_res_tac evaluatePropsTheory.evaluate_sing \\ gs[]
+                \\ rveq \\ gs[extend_env_with_vars_def, namespaceTheory.nsOptBind_def] \\ NO_TAC)
+        )
+      val theAST_opt_backward_sim = store_thm ("theAST_opt_backward_sim",
+        Parse.Term ‘theAST_opt_float_option_noopt ^args = SOME w ⇒
+        theAST_float_returns ^args (compress_word w)’,
+        simp[theAST_opt_float_option_noopt_def, theAST_float_returns_def]
+        \\ rpt gen_tac
+        \\ ntac 5 (TOP_CASE_TAC \\ fs[])
+        \\ strip_tac \\ rveq
+        \\ fs[GSYM local_opt_thm]
+        \\ first_x_assum (mp_then Any assume_tac no_optimisations_eval_sim)
+        \\ fs[]
+        \\ first_x_assum (qspecl_then [‘NoOpt’, ‘empty_state.fp_state.choices’] assume_tac)
+        \\ pop_assum mp_tac \\ impl_tac
+        >- (EVAL_TAC)
+        \\ strip_tac
+        \\ fs[] \\ imp_res_tac noopt_sim_val \\ rveq
+        \\ imp_res_tac noopt_sim_val_fp \\ rveq \\ fs[]
+        \\ qpat_x_assum `evaluate _ _ _ = _` mp_tac
+        \\ qmatch_goalsub_abbrev_tac ‘evaluate emp_upd dEnv
+              [FST(optimise_with_plan theOpts thePlan e_init)] = (emp_res, _)’
+        \\ strip_tac
+        \\ assume_tac (INST_TYPE [“:'a” |-> “:unit”] stos_pass_correct_thm)
+        \\ first_x_assum
+             (qspecl_then [‘emp_upd’, ‘emp_res’, ‘dEnv’, ‘theOpts’, ‘[e_init]’,
+                           ‘[FP_WordTree fp2]’] mp_tac)
+        \\ simp[is_optimise_with_plan_correct_def]
+        \\ impl_tac
+        >- (
+         unabbrev_all_tac
+         \\ fs[empty_state_def, theOpts_def, extend_conf_def, no_fp_opt_conf_def,
+               theAST_env_def, stos_pass_with_plans_def, theAST_plan_result]
+         \\ assume_tac freeVars_list_body \\ gs[theAST_env_def])
+        \\ rpt strip_tac
+        \\ unabbrev_all_tac
+        \\ fs[empty_state_def, semanticPrimitivesTheory.state_component_equality, theAST_env_def]
+        \\ qpat_x_assum ‘evaluate _ _ [ _ ] = _’ mp_tac
+        \\ qmatch_goalsub_abbrev_tac ‘evaluate newSt newEnv _ = _’
+        \\ strip_tac
+        \\ qexists_tac ‘newSt.fp_state.opts’
+        \\ unabbrev_all_tac
+        \\ first_x_assum (mp_then Any (qspec_then ‘0’ assume_tac)
+                      (CONJUNCT1 fpSemPropsTheory.evaluate_add_choices))
+        \\ fs[theOpts_def, no_fp_opt_conf_def, extend_conf_def,
+              config_component_equality, theAST_plan_result]
+        )
+      (* Define a side-condition for the AST *)
+      val theAST_side_def =
+        Define ‘theAST_side ^args = (is_precond_sound ^fvars ^argList ^(theAST_pre_def |> concl |> rhs))’
+      val is_Double_def = Define ‘
+        is_Double [] [] = T ∧
+        is_Double (w1::ws) (d1::ds) = (DOUBLE (Fp_const w1) d1 ∧ is_Double ws ds)’
+      (* Load the necessary constants from the state *)
+      val theAST_v = fetch_v (stringSyntax.fromHOLstring fname) st
+      val theAST_v_def = DB.find ((term_to_string theAST_v)^"_def") |> hd |> #2 |> #1
+      val theAST_spec = store_thm ("theAST_spec",
+        Parse.Term ‘
+        theAST_side ^args ∧
+        is_Double ^argList ^vList  ⇒
+        let result = (theAST_opt_float_option ^args) in
+          (∀ p.
+             app (p:'ffi ffi_proj) ^theAST_v
+                 ^vList
+                 (emp)
+                 (POSTv v.
+                  &DOUBLE_RES result v)) ∧
+          theAST_float_returns (w1,w2,w3) (compress_word (THE result)) ∧
+          real$abs (fp64_to_real (compress_word (THE result)) - theAST_real_spec ^args) ≤ theErrBound’,
+        rpt gen_tac \\ simp[app_def, theAST_side_def, is_Double_def]
+        \\ rpt (disch_then assume_tac)
+        \\ rpt (gen_tac ORELSE (disch_then assume_tac)) \\ fs[]
+        \\ mp_tac errorbounds_AST
+        \\ fs[isOkError_def, option_case_eq, pair_case_eq, getErrorbounds_def, stripFuns_def, PULL_EXISTS]
+        \\ rpt gen_tac
+        \\ TOP_CASE_TAC \\ fs[option_case_eq, pair_case_eq]
+        \\ rpt (gen_tac ORELSE (disch_then assume_tac)) \\ fs[] \\ rveq
+        \\ first_assum (mp_then Any mp_tac CakeML_FloVer_infer_error)
+        \\ fs[checkErrorbounds_succeeds_def, PULL_EXISTS]
+        \\ qpat_x_assum ‘toFloVerCmd _ _ _ = SOME _’
+                        (fn th => disch_then (fn ith => mp_then Any mp_tac ith th) \\ assume_tac th)
+        \\ fs[theAST_pre_def]
+        \\ disch_then (qspecl_then
+                       [‘theAST_env’,
+                        ‘case ^(theAST_opt |> concl |> rhs) of | [Dlet _ _ e] => e’] mp_tac)
+        \\ impl_tac
+        >- fs[stripFuns_def]
+        \\ strip_tac
+        \\ simp[semanticPrimitivesTheory.do_opapp_def, theAST_v_def]
+        \\ reverse conj_tac
+        >- (
+         rpt (pop_assum mp_tac) \\ simp[] \\ rpt (disch_then assume_tac)
+         \\ rveq
+         \\ ‘theAST_opt_float_option_noopt ^args = SOME fp’
+            by (fs[theAST_opt_float_option_noopt_def])
+         \\ imp_res_tac theAST_opt_backward_sim
+         \\ rfs[theAST_opt_float_option_def, theAST_real_spec_def,
+                real_spec_prog_def, theAST_real_spec_def]
+         \\ assume_tac (INST_TYPE [“:'a” |-> “:unit”] stos_pass_real_id_thm)
+         \\ qpat_x_assum `evaluate _ _ [realify _] = _` mp_tac
+         \\ unabbrev_all_tac
+         \\ simp[GSYM local_opt_thm]
+         \\ qmatch_goalsub_abbrev_tac ‘evaluate _ _ [realify (no_optimisations theOpts (FST e_opt))] = _’
+         \\ disch_then (mp_then Any mp_tac evaluate_no_optimisations)
+         \\ fs[]
+         \\ disch_then (qspecl_then [‘NoOpt’, ‘empty_state.fp_state.choices’] mp_tac)
+         \\ impl_tac \\ unabbrev_all_tac
+         >- (EVAL_TAC)
+         \\ qmatch_goalsub_abbrev_tac ‘evaluate emptyWithReals realEnv [realify (FST (optimise_with_plan theOpts thePlan e_init))] = _’
+         \\ strip_tac
+         \\ fs[is_real_id_optimise_with_plan_def]
+         \\ first_x_assum (
+            qspecl_then [ ‘emptyWithReals’, ‘emptyWithReals’, ‘realEnv’, ‘theOpts’, ‘[e_init]’, ‘[Real r]’] mp_tac)
+         \\ simp[MAP]
+         \\ unabbrev_all_tac \\ fs[theAST_plan_result]
+         \\ impl_tac
+         >- (
+          imp_res_tac evaluate_realify_state
+          \\ qpat_x_assum `isPureExp _ ⇒ _ = _` mp_tac
+          \\ impl_tac >- EVAL_TAC
+          \\ strip_tac \\ fs[theOpts_def, no_fp_opt_conf_def])
+         \\ strip_tac \\ rveq
+         \\ irule REAL_LE_TRANS \\ asm_exists_tac \\ fs[])
+        \\ ntac (numArgs-1)
+                (rpt strip_tac \\ once_rewrite_tac [app_basic_def]
+                 \\ simp[semanticPrimitivesTheory.do_opapp_def, set_sepTheory.cond_def]
+                 \\ rpt strip_tac
+                 (* We will return a val but we do not know which one *)
+                 \\ Q.REFINE_EXISTS_TAC ‘Val v’
+                 \\ simp[evaluate_to_heap_def, evaluate_ck_def, terminationTheory.evaluate_def]
+                 \\ ntac 2 (qexists_tac ‘EMPTY’)
+                 \\ fs[emp_def, set_sepTheory.SPLIT_def, cfHeapsBaseTheory.SPLIT3_def,
+                       set_sepTheory.SEP_EXISTS]
+                 \\ simp[Once set_sepTheory.STAR_def]
+                 \\ qexists_tac ‘emp’
+                 \\ rpt (qexists_tac ‘EMPTY’) \\ conj_tac
+                 >- fs[emp_def, set_sepTheory.SPLIT_def, cfHeapsBaseTheory.SPLIT3_def]
+                 \\ conj_tac
+                 >- fs[emp_def])
+        \\ once_rewrite_tac [app_basic_def]
+        \\ simp[semanticPrimitivesTheory.do_opapp_def, set_sepTheory.cond_def]
+        \\ rpt strip_tac
+        \\ Q.REFINE_EXISTS_TAC ‘Val v’
+        \\ simp[DOUBLE_RES_def, theAST_opt_float_option_def]
+        \\ fs[emp_def] \\ rveq
+        \\ qexists_tac ‘EMPTY’
+        \\ rename1 ‘st2heap p st_final’
+        \\ qexists_tac ‘st2heap p st_final’ \\ conj_tac
+        >- fs[emp_def, set_sepTheory.SPLIT_def, cfHeapsBaseTheory.SPLIT3_def]
+        \\ simp[evaluate_to_heap_def, evaluate_ck_def]
+        \\ first_x_assum
+           (mp_then Any mp_tac
+            (INST_TYPE [“:'a”|->“:unit”, “:'b”|->“:'ffi”] pureExpsTheory.isPureExpList_swap_state))
+        \\ disch_then (qspec_then ‘st_final with clock := 0’ mp_tac)
+        \\ impl_tac \\ fs[]
+        >- (unabbrev_all_tac \\ EVAL_TAC)
+        \\ strip_tac \\ qexists_tac ‘0’ \\ fs[extend_env_with_vars_def, DOUBLE_def, theAST_env_def]
+        )
+      (* Some more precreated terms *)
+      val (cl_list, inp_list, inps) =
+        let val (cstStrs, inps) =
+            if numArgs = 1 then
+              (“[cst1s]:mlstring list”, “(cst1s):mlstring”)
+            else if numArgs = 2 then
+              (“[cst1s; cst2s]:mlstring list”, “(cst1s,cst2s):mlstring#mlstring”)
+            else if numArgs = 3 then
+              (“[cst1s; cst2s; cst3s]:mlstring list”,
+              “(cst1s, cst2s, cst3s):mlstring#mlstring#mlstring”)
+            else if numArgs = 4 then
+              (“[cst1s; cst2s; cst3s; cst4s]:mlstring list”,
+              “(cst1s, cst2s, cst3s, cst4s):mlstring#mlstring#mlstring#mlstring”)
+            else if numArgs = 6 then
+              (“[cst1s; cst2s; cst3s; cst4s; cst5s; cst6s]:mlstring list”,
+              “(cst1s, cst2s, cst3s, cst4s, cst5s, cst6s):
+                mlstring#mlstring#mlstring#mlstring#mlstring#mlstring”)
+            else if numArgs = 8 then
+              (“[cst1s; cst2s; cst3s; cst4s; cst5s; cst6s; cst7s; cst8s]:mlstring list”,
+              “(cst1s, cst2s, cst3s, cst4s, cst5s, cst6s, cst7s, cst8s):
+                mlstring#mlstring#mlstring#mlstring#mlstring#mlstring#mlstring#mlstring”)
+            else (* numArgs = 9 *)
+              (“[cst1s; cst2s; cst3s; cst4s; cst5s; cst6s; cst7s; cst8s; cst9s]:mlstring list”,
+              “(cst1s, cst2s, cst3s, cst4s, cst5s, cst6s, cst7s, cst8s, cst9s):
+                mlstring#mlstring#mlstring#mlstring#mlstring#mlstring#mlstring#mlstring#mlstring”)
+        in (EVAL (Parse.Term ‘[fname] ++ ^cstStrs’) |> concl |> rhs, cstStrs, inps)
+        end
+      val all_float_string_def = Define ‘
+        all_float_string [] [] = T ∧
+        all_float_string (s1::ss) (w1::ws) = (is_float_string s1 w1 ∧ all_float_string ss ws)’
+      val main_spec = store_thm ("main_spec",
+        Parse.Term ‘
+        ∀ p.
+        cl = ^cl_list ∧
+        all_float_string ^inp_list ^argList ∧
+        theAST_side ^args ⇒
+        let
+          result = theAST_opt_float_option ^args
+        in
+        app p ^(fetch_v "main" st)
+          [Conv NONE []]
+          (STDIO fs * COMMANDLINE cl)
+          (POSTv uv. &UNIT_TYPE () uv *
+           STDIO (add_stdout fs (mlint$toString (&w2n (compress_word (THE result))))))
+          ∧
+          theAST_float_returns ^args (compress_word (THE result)) ∧
+          real$abs (fp64_to_real (compress_word (THE result)) -
+            theAST_real_spec ^args) ≤ theErrBound’,
+        simp[all_float_string_def] \\ rpt strip_tac
+        \\ first_x_assum $ mp_then Any assume_tac
+                         $ SIMP_RULE std_ss [is_Double_def] (INST_TYPE [“:'ffi”|->“:'a”] theAST_spec)
+        >- (
+         xcf "main" st
+         (* let for unit value *)
+         \\ xlet_auto >- (xcon \\ xsimpl)
+         \\ ‘^(numSyntax.term_of_int (numArgs+1)) = LENGTH cl’ by (rveq \\ fs[])
+         \\ rveq
+         \\ xlet_auto_spec (SOME reader_spec)
+         >- (xsimpl \\ qexists_tac ‘emp’ \\ xsimpl
+             \\ qexists_tac ‘fs’ \\ xsimpl)
+         \\ xmatch
+         \\ fs[PAIR_TYPE_def] \\ reverse conj_tac
+         >- (EVAL_TAC \\ fs[])
+         \\ rveq \\ fs[is_float_string_def] \\ rveq
+         \\ ntac numArgs (
+           last_x_assum (mp_then Any mp_tac intToFP_spec)
+           \\ disch_then (fn ith => last_x_assum $ mp_then Any mp_tac ith)
+           \\ disch_then drule
+           \\ disch_then (qspecl_then [‘p’, ‘fs’] assume_tac)
+           \\ xlet_auto
+           >- (xsimpl \\ qexists_tac ‘emp’ \\ xsimpl
+               \\ qexists_tac ‘fs’ \\ xsimpl)
+           \\ qpat_x_assum `app _ intToFP_v _ _ _` kall_tac)
+         \\ first_x_assum drule
+         \\ rpt (disch_then drule) \\ strip_tac
+         \\ xlet_auto >- xsimpl
+         \\ qpat_x_assum ‘DOUBLE_RES _ _’ mp_tac
+         \\ simp[DOUBLE_RES_def] \\ TOP_CASE_TAC \\ fs[]
+         \\ rpt strip_tac \\ rveq
+         \\ qmatch_goalsub_abbrev_tac ‘compress_word f’
+         \\ xlet ‘POSTv v. &WORD (compress_word f) v * STDIO fs’
+         >- (
+          fs[cf_fptoword_def, cfHeapsTheory.local_def, cfNormaliseTheory.exp2v_def,
+             cfTheory.app_fptoword_def]
+          \\ rpt strip_tac
+          \\ fs[WORD_def]
+          \\ qexists_tac ‘STDIO fs’ \\ qexists_tac ‘emp’
+          \\ fs[set_sepTheory.STAR_def]
+          \\ qexists_tac ‘POSTv v. &WORD (compress_word f) v * STDIO fs’ \\ rpt conj_tac
+          >- (
+           qexists_tac ‘h’ \\ qexists_tac ‘EMPTY’ \\ fs[SPLIT_def, emp_def])
+          >- (
+           fs[DOUBLE_def, set_sepTheory.SEP_IMP_def]
+           \\ rpt strip_tac \\ fs[set_sepTheory.cond_def, set_sepTheory.STAR_def]
+           \\ qexists_tac ‘s’ \\ fs[SPLIT_def])
+          \\ xsimpl \\ rveq \\ rpt strip_tac
+          \\ fs[set_sepTheory.SEP_IMP_def, set_sepTheory.STAR_def] \\ rpt strip_tac
+          \\ qexists_tac ‘s’ \\ qexists_tac ‘EMPTY’
+          \\ fs[SPLIT_def, GC_def] \\ conj_tac
+          >- (rveq \\ rewrite_tac [CONJ_ASSOC]
+              \\ once_rewrite_tac [CONJ_COMM] \\ asm_exists_tac \\ fs[]
+              \\ qexists_tac ‘EMPTY’
+              \\ fs[set_sepTheory.cond_def, WORD_def])
+          \\ fs[set_sepTheory.SEP_EXISTS] \\ qexists_tac ‘emp’ \\ fs[emp_def])
+         \\ xapp \\ xsimpl)
+        \\ fs[DOUBLE_def]
+        )
+      val main_whole_prog_spec = store_thm ("main_whole_prog_spec",
+        Parse.Term ‘
+        cl = ^cl_list ∧
+        all_float_string ^inp_list ^argList ∧
+        theAST_side ^args ⇒
+        whole_prog_spec ^(fetch_v "main" st) cl fs
+        NONE
+        ((=)
+         (add_stdout fs (mlint$toString (&w2n (compress_word (THE (theAST_opt_float_option ^args)))))))
+        ∧
+        theAST_float_returns ^args (compress_word (THE (theAST_opt_float_option ^args))) ∧
+        real$abs (fp64_to_real (compress_word (THE (theAST_opt_float_option ^args))) -
+                  theAST_real_spec ^args) ≤ theErrBound’,
+        simp[whole_prog_spec_def]
+        \\ qmatch_goalsub_abbrev_tac`fs1 = _ with numchars := _`
+        \\ rpt (strip_tac)
+        \\ qspec_then ‘(basis_proj1, basis_proj2)’ mp_tac main_spec
+        \\ impl_tac \\ fs[]
+        \\ strip_tac
+        \\ qexists_tac`fs1`
+        \\ simp[Abbr`fs1`,GSYM add_stdo_with_numchars,with_same_numchars]
+        \\ first_x_assum (fn main_spec => irule (MP_CANON (MATCH_MP app_wgframe main_spec)))
+        \\ xsimpl
+        )
+      (* Put it all together into a theorem for the final spec proof *)
+      val spec = main_whole_prog_spec;
+      val name = "main";
+      val (prog_rewrite, semantics_prog_thm) = mk_whole_prog_spec_thm spec name (get_ml_prog_state());
+      val theAST_prog_tm = rhs (concl prog_rewrite);
+      val theAST_prog_def = Define`theAST_prog = ^theAST_prog_tm`;
+      val full_semantics_prog_thm =
+            CONJUNCT2 (SIMP_RULE std_ss [cfSupportTheory.IMP_SPLIT] main_whole_prog_spec)
+                    |> SIMP_RULE std_ss [GSYM cfSupportTheory.IMP_SPLIT, GSYM AND_IMP_INTRO]
+                    |> UNDISCH_ALL
+                    |> (fn th => LIST_CONJ [semantics_prog_thm, th])
+                    |> DISCH_ALL |> SIMP_RULE std_ss [];
+      val theAST_semantics =
+        full_semantics_prog_thm |> ONCE_REWRITE_RULE[GSYM theAST_prog_def]
+        |> DISCH_ALL |> SIMP_RULE std_ss [AND_IMP_INTRO,GSYM CONJ_ASSOC];
+      val theAST_semantics_side_def = Define ‘
+        theAST_semantics_side ^inps ^args ⇔
+          all_float_string ^inp_list ^argList ∧
+          theAST_side ^args’
+      val theAST_semantics_final = store_thm ("theAST_semantics_final",
+        Parse.Term ‘theAST_semantics_side ^inps ^args ∧ init_ok (^cl_list,fs) ⇒
+        ∃ (w:word64).
+          CakeML_evaluates_and_prints (^cl_list,fs,theAST_prog) (toString w) ∧
+          theAST_float_returns ^args w ∧
+          real$abs (fp64_to_real w - theAST_real_spec ^args) ≤ theErrBound’,
+        rpt strip_tac
+        \\ fs[init_ok_def, CakeML_evaluates_and_prints_def, theAST_semantics_side_def]
+        \\ first_x_assum (mp_then Any mp_tac theAST_semantics)
+        \\ rpt (disch_then drule) \\ fs[]
+        \\ disch_then drule \\ strip_tac
+        \\ qexists_tac ‘compress_word (THE (theAST_opt_float_option ^args))’ \\ fs[]
+        \\ asm_exists_tac \\ fs[toString_def]
+        )
+      in theAST_semantics_final end
   in () end;
 
 end;
